\section{Vectores}


\begin{enumerate}
    \item Siendo los vectores $\vec{a} = (4; 5; 6),\;\; \vec{b} = (-2; -5; -2),\;\; \vec{c} = \left(\pi; 0; \sqrt{7} \right)$, calcular: 
    $$\left| \left( (\vec{a} \bullet \vec{b}) \cdot \vec{a} + \vec{b} \right) \times \vec{c} \right|$$

    \item Siendo los vectores $\vec{a} = (-4; 0; 2),\;\; \vec{b} = (1; 2; 3),\;\; \vec{c} = \left(\sqrt{2}\pi; -\sqrt{5}; 0 \right)$, calcular:
    $$
    \left( \left| \vec{c} \right|+ \vec{a} \bullet \vec{b}
    \right) \cdot (\vec{a} \times \vec{b})
    $$


    \item Siendo los vectores $\vec{a} = (-5; 3; -1),\;\; \vec{b} = (-\sqrt{7}; 0; 3),\;\; \vec{c} = \left(-\pi; \sqrt{5}; 1 \right)$, calcular:
    $$
    \left|
    \left( \vec{a} \bullet \vec{b} \right) \cdot
    (\vec{a} \times {b})
    + \left| \vec{b}\right| \cdot
    (\vec{c} \times \vec{a})
    \right|
    $$

    \item Siendo los vectores $\vec{a} = (2; -4; -\pi),\;\; \vec{b} = (1; 0; -1),\;\; \vec{c} = \left(\pi; \sqrt{5}; 0 \right)$, calcular:
    $$
    \left|
    5 \cdot \left(
        \vec{c} + \vec{a} \times \vec{b}
    \right) -
    \vec{c}
    \right|
    $$

    \item Siendo los vectores $\vec{a} = (3; -4; 5),\;\; \vec{b} = (2; 0; -2),\;\; \vec{c} = \left(1; 0; \sqrt{2} \right)$, calcular:
    $$
    \left( \vec{a} + \vec{b}  \right) \times
    \left( \left| \vec{c} \right| \cdot \vec{c} \right)
    $$

    \item Siendo los vectores $\vec{a} = (1; 0; -1),\;\; \vec{b} = (1; 2; 3),\;\; \vec{c} = \left(0; -5; \sqrt{2} \right)$, calcular:
    $$
    \left( \vec{a} + \vec{b} - \vec{c}  \right) \times
    \left( \left| \vec{c} \right| \cdot \vec{c} \right)
    $$
\end{enumerate}